

Lecture 9: Random Matrices III

9 Rigorous Upper Bound

Recap: A Gaussian orthogonal ensemble (GOE) matrix $J \in \mathbb{R}^{n \times n}$ is a random symmetric matrix with entries distributed as

$$J_{ij} = J_{ji}, \quad J_{ij} \stackrel{\text{i.i.d.}}{\sim} \mathcal{N}\left(0, \frac{1}{n}\right) \text{ for } i < j, \quad J_{ii} \stackrel{\text{i.i.d.}}{\sim} \mathcal{N}\left(0, \frac{2}{n}\right) \text{ for } i = 1, \dots, n.$$

In the previous two lectures, we analyzed the largest eigenvalue $\lambda_{\max}(J)$ and derived

$$\lim_{n \rightarrow \infty} \mathbb{E}[\lambda_{\max}(J)] = 2$$

using the replica method.

In this lecture, we provide a rigorous proof of the corresponding upper bound:

$$\mathbb{E}[\lambda_{\max}(J)] \leq 2.$$

9.1 Motivation

For a GOE matrix J , consider the collection¹

$$g = (\langle x, Jx \rangle)_{x \in S^{n-1}}, \quad S^{n-1} = \{x \in \mathbb{R}^n : \|x\|_2 = 1\},$$

which defines a mean-zero Gaussian process. The largest eigenvalue of J can then be written as

$$\lambda_{\max}(J) = \max_{x \in S^{n-1}} \langle x, Jx \rangle =: \max_{x \in \mathcal{X}} g_x,$$

where $\mathcal{X} = S^{n-1}$. Our goal is to derive a uniform upper bound for this Gaussian process:

$$\mathbb{E} \left[\max_{x \in \mathcal{X}} g_x \right] \leq ?.$$

Since the exact value of $\mathbb{E}[\max_{x \in \mathcal{X}} g_x]$ in the GOE case is difficult to compute, our strategy is to construct a stochastically dominating Gaussian process h on the same index set \mathcal{X} such that

$$\mathbb{E} \left[\max_{x \in \mathcal{X}} g_x \right] \leq \mathbb{E} \left[\max_{x \in \mathcal{X}} h_x \right],$$

and $\mathbb{E}[\max_{x \in \mathcal{X}} h_x]$ is tractable to compute.

We begin with a general comparison inequality for Gaussian processes, which intuitively states that a process exhibiting greater variability has a larger expected maximum. We will then apply this result to identify a suitable dominating process for the GOE case and complete the rigorous upper bound.

¹In class, we used an asymmetric version of the process which slightly breaks some calculations. These notes have the fixed and simplified version.

Theorem 1 (Sudakov-Fernique Inequality). *Let $(g_x)_{x \in \mathcal{X}}$ and $(h_x)_{x \in \mathcal{X}}$ be two mean-zero Gaussian processes on the same index set \mathcal{X} . Suppose that for all $x, y \in \mathcal{X}$,*

$$\text{Var}(g_x - g_y) \leq \text{Var}(h_x - h_y).$$

Then

$$\mathbb{E} \left[\log \sum_{x \in \mathcal{X}} \exp(g_x) \right] \leq \mathbb{E} \left[\log \sum_{x \in \mathcal{X}} \exp(h_x) \right], \quad (1)$$

$$\mathbb{E} \left[\max_{x \in \mathcal{X}} g_x \right] \leq \mathbb{E} \left[\max_{x \in \mathcal{X}} h_x \right]. \quad (2)$$

Example 1. Consider two Gaussian random vectors

$$g \sim \mathcal{N}(0, \mathbb{1}\mathbb{1}^\top), \quad h \sim \mathcal{N}(0, I_n),$$

which can also be viewed as two Gaussian processes indexed by the finite set $\mathcal{X} = [n]$.

For any $i \neq j \in [n]$,

$$\text{Var}(g_i - g_j) = 0, \quad \text{Var}(h_i - h_j) = 2.$$

By the Sudakov-Fernique inequality,

$$\mathbb{E} \left[\max_{i \in [n]} g_i \right] \leq \mathbb{E} \left[\max_{i \in [n]} h_i \right].$$

In fact, for the random vector g , all coordinates are identical:

$$g_1 = g_2 = \dots = g_n, \quad g_1 \sim \mathcal{N}(0, 1), \quad \mathbb{E} \left[\max_{i \in [n]} g_i \right] = \mathbb{E}[g_1] = 0.$$

In contrast, for h , the components $\{h_i\}_{i=1}^n$ are i.i.d $\mathcal{N}(0, 1)$ random variables, and there exists a small absolute constant $c > 0$ such that

$$\mathbb{E} \max_{i \in [n]} h_i \geq c\sqrt{\log n}.$$

Intuitively, the randomness in g arises from a single standard Gaussian variable shared across all coordinates, whereas the randomness in h comes from n independent standard Gaussian variables, which aligns with the intuition behind the Sudakov-Fernique inequality.

9.2 Gaussian interpolation

The proof of the Sudakov-Fernique inequality relies on the Gaussian interpolation trick. Let $(g_x)_{x \in \mathcal{X}}$ and $(h_x)_{x \in \mathcal{X}}$ be independent mean-zero Gaussian processes on the same index set \mathcal{X} . For any $x \in \mathcal{X}$, define the interpolating process as

$$G_x(t) = \sqrt{t}g_x + \sqrt{1-t}h_x, \quad t \in [0, 1].$$

Then $G_x(0) = h_x$, $G_x(1) = g_x$, and

$$\text{Var}(G_x(t)) = t \text{Var}(g_x) + (1-t) \text{Var}(h_x).$$

The motivation for the Gaussian interpolation trick is that, instead of proving the conclusions of Theorem 1 directly, one can show that the corresponding quantities of interest (such as the expected maximum) associated with the interpolated process $G_x(t)$ are decreasing in t . This monotonicity immediately implies the desired inequalities. The elegance of this method is that this can be investigated locally by considering the derivative with respect to t .

Before proceeding to the proof of Theorem 1 via the Gaussian interpolation trick, we introduce a useful lemma called Gaussian integration by parts.

Lemma 1 (Gaussian Integration By Parts). *Let $X \sim \mathcal{N}(0, \Sigma)$, where Σ is an $n \times n$ covariance matrix. Then for any differentiable function $f : \mathbb{R}^n \rightarrow \mathbb{R}$,*

$$\mathbb{E}[X_i f(X)] = \sum_{j=1}^n \Sigma_{ij} \mathbb{E} \left[\frac{\partial f}{\partial x_j}(X) \right],$$

assuming the expectations above exist and are finite.

Proof. We first establish the result in one dimension. Let $\xi \sim \mathcal{N}(0, 1)$, for any differentiable function $\varphi : \mathbb{R} \rightarrow \mathbb{R}$ with compact support,

$$\begin{aligned} \mathbb{E}[\varphi'(\xi)] &= \frac{1}{\sqrt{2\pi}} \int_{-\infty}^{\infty} \varphi'(x) e^{-\frac{x^2}{2}} dx \\ &= \frac{1}{\sqrt{2\pi}} \varphi(x) e^{-\frac{x^2}{2}} \Big|_{-\infty}^{+\infty} + \frac{1}{\sqrt{2\pi}} \int_{-\infty}^{\infty} x \varphi(x) e^{-\frac{x^2}{2}} dx \\ &= \mathbb{E}[\xi \varphi(\xi)] \end{aligned}$$

by integration by parts. By an approximation argument, the result extends to all φ such that $\xi \varphi(\xi)$ and $\varphi'(\xi)$ are integrable.

Write $X = \Sigma^{1/2} Z$, where $Z \sim \mathcal{N}(0, I_n)$. Then $X_i = \sum_{k=1}^n \Sigma_{ik}^{1/2} Z_k$, and hence

$$\mathbb{E}[X_i f(X)] = \sum_{k=1}^n \Sigma_{ik}^{1/2} \mathbb{E}[Z_k f(\Sigma^{1/2} Z)] = \sum_{k=1}^n \Sigma_{ik}^{1/2} \mathbb{E}[\mathbb{E}[Z_k f(\Sigma^{1/2} Z) \mid Z_{-k}]],$$

where $Z_{-k} = \{Z_j\}_{j \neq k}$.

Since $\{Z_k\}_{k=1}^n$ are independent, we have $Z_k \mid Z_{-k} \sim \mathcal{N}(0, 1)$. Applying the one-dimensional result together with the chain rule gives

$$\mathbb{E}[Z_k f(\Sigma^{1/2} Z) \mid Z_{-k}] = \sum_{j=1}^n \Sigma_{jk}^{1/2} \mathbb{E} \left[\frac{\partial f}{\partial x_j}(\Sigma^{1/2} Z) \mid Z_{-k} \right].$$

Therefore,

$$\begin{aligned} \mathbb{E}[X_i f(X)] &= \sum_{k=1}^n \Sigma_{ik}^{1/2} \sum_{j=1}^n \Sigma_{jk}^{1/2} \mathbb{E} \left[\frac{\partial f}{\partial x_j}(\Sigma^{1/2} Z) \right] \\ &= \sum_{j=1}^n \left(\sum_{k=1}^n \Sigma_{ik}^{1/2} \Sigma_{kj}^{1/2} \right) \mathbb{E} \left[\frac{\partial f}{\partial x_j}(\Sigma^{1/2} Z) \right] \\ &= \sum_{j=1}^n \Sigma_{ij} \mathbb{E} \left[\frac{\partial f}{\partial x_j}(X) \right], \end{aligned}$$

which completes the proof. □

9.3 Proof of the Sudakov-Fernique inequality

Proof of Theorem 1. If for any $t \in (0, 1)$ and $\beta > 0$,

$$\frac{d}{dt} \mathbb{E} \left[\log \sum_{x \in \mathcal{X}} \exp(\beta G_x(t)) \right] \leq 0, \tag{3}$$

then integrating over t yields

$$\begin{aligned}\mathbb{E} \left[\log \sum_{x \in \mathcal{X}} \exp(\beta G_x(1)) \right] &= \mathbb{E} \left[\log \sum_{x \in \mathcal{X}} \exp(\beta G_x(0)) \right] + \int_0^1 \frac{d}{dt} \mathbb{E} \left[\log \sum_{x \in \mathcal{X}} \exp(\beta G_x(t)) \right] dt \\ &\leq \mathbb{E} \left[\log \sum_{x \in \mathcal{X}} \exp(\beta G_x(0)) \right].\end{aligned}$$

Taking $\beta = 1$ gives the first inequality in 1. Moreover, since

$$\lim_{\beta \rightarrow \infty} \frac{1}{\beta} \log \sum_{x \in \mathcal{X}} \exp(\beta G_x(t)) = \max_{x \in \mathcal{X}} G_x(t),$$

letting $\beta \rightarrow \infty$ yields the second inequality in 2.

Therefore, it suffices to prove that for any $t \in (0, 1)$ and $\beta > 0$, inequality 3 holds. We have

$$\frac{d}{dt} G_x(t) = \frac{1}{2} \left(\frac{g_x}{\sqrt{t}} - \frac{h_x}{\sqrt{1-t}} \right),$$

and hence

$$\begin{aligned}\frac{d}{dt} \log \sum_{x \in \mathcal{X}} \exp(\beta G_x(t)) &= \frac{\sum_{x \in \mathcal{X}} \frac{d}{dt} \exp(\beta G_x(t))}{\sum_{x \in \mathcal{X}} \exp(\beta G_x(t))} \\ &= \frac{\beta}{2} \cdot \frac{\sum_{x \in \mathcal{X}} \exp(\beta G_x(t)) \cdot (g_x/\sqrt{t} - h_x/\sqrt{1-t})}{\sum_{x \in \mathcal{X}} \exp(\beta G_x(t))}\end{aligned}$$

Since g and h are independent, conditioning on h leaves g as the same Gaussian process. Conditioned on any realization of h , define the softmax weights

$$\psi_{h,x}(g) = \frac{\exp(\beta G_x(t))}{\sum_{x \in \mathcal{X}} \exp(\beta G_x(t))}.$$

By Lemma 1, for each fixed x

$$\begin{aligned}\mathbb{E} [\psi_{h,x}(g) \cdot g_x | h] &= \sum_{y \in \mathcal{X}} \text{Cov}(g_x, g_y) \mathbb{E} \left[\frac{\partial \psi_{h,x}}{\partial g_y}(g) \middle| h \right] \\ &= \sum_{y \in \mathcal{X}} \text{Cov}(g_x, g_y) \mathbb{E} \left[\frac{\mathbb{1}\{y = x\} \cdot \beta \sqrt{t} \exp(\beta G_y(t)) \sum_{x' \in \mathcal{X}} \exp(\beta G_{x'}(t))}{(\sum_{x' \in \mathcal{X}} \exp(\beta G_{x'}(t)))^2} \right. \\ &\quad \left. - \frac{\beta \sqrt{t} \exp(\beta G_x(t)) \exp(\beta G_y(t))}{(\sum_{x' \in \mathcal{X}} \exp(\beta G_{x'}(t)))^2} \middle| h \right] \\ &= \beta \sqrt{t} \left(\text{Cov}(g_x, g_x) \sum_{y \in \mathcal{X}} \mathbb{E} \left[\frac{\exp(\beta G_x(t) + \beta G_y(t))}{(\sum_{x' \in \mathcal{X}} \exp(\beta G_{x'}(t)))^2} \middle| h \right] \right. \\ &\quad \left. - \sum_{y \in \mathcal{X}} \text{Cov}(g_x, g_y) \mathbb{E} \left[\frac{\exp(\beta G_x(t) + \beta G_y(t))}{(\sum_{x' \in \mathcal{X}} \exp(\beta G_{x'}(t)))^2} \middle| h \right] \right)\end{aligned}$$

Define

$$H(x, y) = \mathbb{E} \left[\frac{\exp(\beta G_x(t) + \beta G_y(t))}{(\sum_{x' \in \mathcal{X}} \exp(\beta G_{x'}(t)))^2} \right] > 0.$$

Then by the law of total expectation,

$$\begin{aligned}
\mathbb{E} \left[\frac{\beta}{2} \sum_{x \in \mathcal{X}} \psi_{h,x}(g) \cdot \frac{g_x}{\sqrt{t}} \right] &= \frac{\beta^2}{2} \sum_{x \in \mathcal{X}} \sum_{y \in \mathcal{X}} (\text{Cov}(g_x, g_x) - \text{Cov}(g_x, g_y)) \cdot H(x, y) \\
&= \frac{\beta^2}{2} \sum_{x \neq y} (\text{Cov}(g_x, g_x) - \text{Cov}(g_x, g_y)) \cdot H(x, y) \\
&= \frac{\beta^2}{4} \sum_{x \neq y} (\text{Cov}(g_x, g_x) - 2 \text{Cov}(g_x, g_y) + \text{Cov}(g_y, g_y)) \cdot H(x, y) \\
&= \frac{\beta^2}{4} \sum_{x \neq y} \text{Var}(g_x - g_y) \cdot H(x, y).
\end{aligned}$$

By a symmetric argument for the h -term, we obtain

$$\begin{aligned}
\frac{d}{dt} \mathbb{E} \left[\log \sum_{x \in \mathcal{X}} \exp(\beta G_x(t)) \right] &= \frac{\beta^2}{4} \sum_{x \neq y} (\text{Var}(g_x - g_y) - \text{Var}(h_x - h_y)) \cdot H(x, y) \\
&\leq 0,
\end{aligned}$$

where the last inequality follows from the assumption. This verifies inequality (3) and thus completes the proof of Theorem 1. \square

9.4 Application: sharp upper bound for GOE

In our GOE case, we compute the variance of the Gaussian process g . For any $x \in \mathcal{X}$ and $y \in \mathcal{X}$,

$$\begin{aligned}
\text{Var}(g_x - g_y) &= \text{Var}(\langle x, Jx \rangle - \langle y, Jy \rangle) \\
&= \text{Var}(\langle J, xx^\top - yy^\top \rangle) \\
&= \frac{\|xx^\top - yy^\top\|_F^2 + \text{tr}((xx^\top - yy^\top)^2)}{n} \\
&= \frac{4(1 - \langle x, y \rangle^2)}{n}.
\end{aligned}$$

To apply the Sudakov–Fernique inequality, we construct another mean-zero Gaussian process with larger pairwise variance. For any $x = (u, v) \in \mathcal{X}$, define

$$h_x = \frac{2\langle Z, x \rangle}{\sqrt{n}},$$

where $Z \sim \mathcal{N}(0, I_n)$. Then for $x \in \mathcal{X}$ and $y \in \mathcal{X}$,

$$\begin{aligned}
\text{Var}(h_x - h_y) &= \text{Var}\left(\frac{2\langle Z, x - y \rangle}{\sqrt{n}}\right) \\
&= \frac{4\|x - y\|_2^2}{n} \\
&= \frac{8(1 - \langle x, y \rangle)}{n}.
\end{aligned}$$

Since $x, y \in S^{n-1}$, we have $t := \langle x, y \rangle \leq 1$. Hence

$$\begin{aligned}
\text{Var}(h_x - h_y) - \text{Var}(g_x - g_y) &= \frac{4(2 - 2t - 1 + t^2)}{n} \\
&= \frac{4(1 - t)^2}{n} \\
&\geq 0.
\end{aligned}$$

By the Sudakov-Fernique inequality,

$$\mathbb{E} \left[\max_{x \in \mathcal{X}} g_x \right] \leq \mathbb{E} \left[\max_{x \in \mathcal{X}} h_x \right] = \mathbb{E} \left[\frac{2\|Z\|_2}{\sqrt{n}} \right] \leq 2,$$

where the last inequality follows from

$$\mathbb{E} [\|Z\|_2] = \mathbb{E} \left[\sqrt{\|Z\|_2^2} \right] \leq \sqrt{\mathbb{E} [\|Z\|_2^2]} = \sqrt{n},$$

by Jensen's inequality. Consequently,

$$\mathbb{E} [\lambda_{\max}(J)] = \mathbb{E} \left[\max_{x \in \mathcal{X}} g_x \right] \leq 2,$$

which is the desired upper bound.